more work on optimizations

tutorial/AsmOptimization.v
@@ -40,8 +40,6 @@ Open Scope cat_scope.
 (* end hide *)
 
 
-
-
 (* optimizations ------------------------------------------------------------ *)
 
 (** A (simple) optimization is just a function from asm units to asm units. *)
@@ -56,9 +54,312 @@ Definition optimization {A B} := asm A B -> asm A B.
       differences in the state.  Those optimizations would require
       more contextual information.
 *)
+
+(** We define an appropriate notion of equivalence on these state components.
+    This will be useful for defining optimizations at the [Asm] level. *)
+Definition EQ_registers (regs1 regs2 : registers) : Prop :=
+  forall k v, alist_In k regs1 v <-> alist_In k regs2 v.
+
+Definition EQ_memory (mem1 mem2 : memory) : Prop :=
+  forall k v, alist_In k mem1 v <-> alist_In k mem2 v.
+
+Global Instance EQ_registers_refl : Reflexive EQ_registers.
+  Proof.
+    red. intros. unfold EQ_registers. tauto.
+  Qed.    
+
+Global Instance EQ_registers_sym : Symmetric EQ_registers.
+  Proof.
+    repeat intro. 
+    split; intros; apply H; assumption.
+  Qed.
+
+Global Instance EQ_registers_trans : Transitive EQ_registers.
+  Proof.
+    repeat intro. 
+    unfold EQ_registers in *.
+    split; intros.
+    - apply H0. apply H. assumption.
+    - apply H. apply H0. assumption.
+  Qed.
+  
+Global Instance EQ_registers_eqv : Equivalence EQ_registers.
+constructor; typeclasses eauto. 
+  
+  
+Global Instance EQ_memory_refl : Reflexive EQ_memory.
+Proof.
+  red. intros. unfold EQ_memory. tauto.
+Qed.    
+
+Global Instance EQ_memory_sym : Symmetric EQ_memory.
+  Proof.
+    repeat intro. 
+    split; intros; apply H; assumption.
+  Qed.
+
+Global Instance EQ_memory_trans : Transitive EQ_memory.
+  Proof.
+    repeat intro. 
+    unfold EQ_registers in *.
+    split; intros.
+    - apply H0. apply H. assumption.
+    - apply H. apply H0. assumption.
+  Qed.
+
+Global Instance EQ_memory_eqv : Equivalence EQ_memory.
+Proof.
+constructor; typeclasses eauto. 
+Qed.
+
+Inductive rel_asm {B} : memory * (registers * B) -> memory * (registers * B) -> Prop :=
+|rel_asm_ctr : forall b mem1 mem2 regs1 regs2
+                 (HMem : EQ_memory mem1 mem2)
+                 (HReg : EQ_registers regs1 regs2),
+    rel_asm (mem1, (regs1, b)) (mem2, (regs2, b)).
+
+Global Instance rel_asm_refl {B} : Reflexive (@rel_asm B).
+Proof.
+  repeat intro.
+  destruct x as [m [r b]].
+  constructor; reflexivity.
+Qed.  
+
+Global Instance rel_asm_sym {B} : Symmetric (@rel_asm B).
+Proof.
+  repeat intro.
+  inversion H.
+  subst.
+  constructor; symmetry; assumption.
+Qed.  
+
+Global Instance rel_asm_trans {B} : Transitive (@rel_asm B).
+Proof.
+  repeat intro.
+  inversion H.
+  inversion H0.
+  subst. inversion H3. subst.
+  constructor; eapply transitivity; eassumption.
+Qed.
+
+Global Instance rel_asm_eqv {B} : Equivalence (@rel_asm B).
+Proof.
+  constructor; typeclasses eauto.
+Qed.
+
+Global Instance eutt_rel_asm_refl {E R} {r : R -> R -> Prop} `{Reflexive _ r} : Reflexive (@eutt E R R r).
+Proof.
+  (* SAZ: Should this be in the library? *)
+Admitted.
+
+Global Instance eutt_rel_asm_sym {E R} {r : R -> R -> Prop} `{Symmetric _ r} : Symmetric (@eutt E R R r).
+Proof.
+  (* SAZ: Should this be in the library? *)
+Admitted.
+
+Global Instance eutt_rel_asm_trans {E R} {r : R -> R -> Prop} `{Transitive _ r} : Transitive (@eutt E R R r).
+Proof.
+  (* SAZ: Should this be in the library? *)
+Admitted.
+
+Global Instance eutt_rel_asm_equiv {E R} {r : R -> R -> Prop} `{Equivalence _ r} : Equivalence (@eutt E R R r).
+Proof.
+  constructor; typeclasses eauto.
+Qed.
+
+
+(** The definition [interp_asm] also induces a notion of equivalence (open)
+    _asm_ programs, which is just the equivalence of the ktree category *)
+Definition eq_asm_denotations_EQ {E A B} (t1 t2 : Kleisli (itree (Reg +' Memory +' E)) A B) : Prop :=
+  forall a mem1 mem2 regs1 regs2,
+    EQ_memory mem1 mem2 ->
+    EQ_registers regs1 regs2 ->
+    (eutt rel_asm)
+      (interp_asm (t1 a) mem1 regs1)
+      (interp_asm (t2 a) mem2 regs2).
+
+Definition eq_asm_EQ {A B} (p1 p2 : asm A B) : Prop :=
+  eq_asm_denotations_EQ (denote_asm p1) (denote_asm p2).
+
 Definition optimization_correct A B (opt:optimization) :=
   forall (p : asm A B),
-    eq_asm p (opt p).
+    eq_asm_EQ p (opt p).
+
+Definition EQ_asm {E A} (f g : memory -> registers -> itree E _) : Prop :=
+  forall mem1 mem2 regs1 regs2,
+    EQ_memory mem1 mem2 ->
+    EQ_registers regs2 regs2 ->
+    eutt (@rel_asm A) (f mem1 regs1) (g mem2 regs2).
+
+Infix "≡" := EQ_asm (at level 70).
+
+
+(* SAZ: I'm not sure that this can be proved without coinduction on t.
+   It probably belongs in the state part of the library, along with the
+   appropriate definition of eutt, etc.
+
+   It also depends crucially on the fact that the handlers respect
+   the equivalence on the state maps.     
+*)
+Lemma interp_asm_id:
+  forall (t : itree (Reg +' Memory +' Exit) unit),
+    (interp_asm t) ≡ (interp_asm t).
+Proof.
+  intros t mem1 mem2 regs1 regs2 H1 H2.
+  unfold interp_asm.
+  unfold run_map.
+  unfold interp_state.
+  pose proof @eutt_interp.
+Admitted.    
+
+
+Lemma interp_asm_ret_tt : forall (t : itree (Reg +' Memory +' Exit) unit),
+    (interp_asm t) ≡ (interp_asm (t ;; Ret tt)).
+Proof.
+  intros t mem1 mem2 regs1 regs2 H1 H2.
+  rewrite interp_asm_bind.
+  rewrite <- bind_ret2 at 1.
+  eapply eutt_clo_bind.
+  { apply interp_asm_id; auto. }
+  intros.
+  inversion H; subst.
+
+  unfold interp_asm.
+  unfold run_map.
+  rewrite interp_ret.
+  do 2 rewrite interp_state_ret.
+  apply eqit_Ret. destruct b. assumption.
+Qed.
+
+Definition lookup_default {K V} `{Map K V} k v m :=
+  match Maps.lookup k m with
+  | Some v' => v'
+  | None => v
+  end.
+
+Lemma interp_asm_ret {E A} (x:A) mem reg :
+  interp_asm (Ret x) mem reg ≈ (Ret (mem, (reg, x)) : itree E _).
+Proof.
+  unfold interp_asm, run_map.
+  rewrite interp_ret.
+  repeat rewrite interp_state_ret.
+  reflexivity.
+Qed.
+
+Lemma interp_asm_GetReg {E A} f r mem reg :
+  @eutt E _ _ (@rel_asm A)
+       (interp_asm (val <- trigger (GetReg r) ;; f val) mem reg)
+       ((interp_asm (f (lookup_default r 0 reg))) mem reg).
+Proof.
+  unfold interp_asm, run_map.
+  rewrite interp_bind.
+  unfold trigger.
+  rewrite interp_vis. rewrite tau_eutt.
+  unfold subevent, resum, ReSum_inl, resum, ReSum_id, id_. cbn.
+  setoid_rewrite interp_ret.
+  rewrite bind_bind.
+  setoid_rewrite bind_ret.
+  repeat rewrite interp_state_bind.
+  unfold Id_IFun.
+  unfold CategoryOps.cat, Cat_Handler, Handler.cat. cbn.
+  unfold inl_, Inl_sum1_Handler, Handler.inl_, Handler.htrigger.
+  unfold lookup_def.
+  rewrite interp_bind.
+  setoid_rewrite interp_trigger. rewrite tau_eutt.
+  setoid_rewrite interp_ret.
+  repeat rewrite interp_state_bind.
+  repeat setoid_rewrite interp_state_ret.
+  rewrite interp_state_trigger. rewrite tau_eutt.
+  cbn .
+  rewrite interp_state_ret.
+  repeat rewrite bind_ret.
+  cbn.
+  unfold lookup_default.
+  unfold lookup, Map_alist. reflexivity.
+Qed.  
+
+Lemma interp_asm_SetReg {E A} f r v mem reg :
+  @eutt E _ _ (@rel_asm A)
+       (interp_asm (trigger (SetReg r v) ;; f) mem reg)
+       ((interp_asm f) mem (Maps.add r v reg)).
+Proof.
+  unfold interp_asm, run_map.
+  rewrite interp_bind.
+  unfold trigger.
+  rewrite interp_vis. rewrite tau_eutt.
+  unfold subevent, resum, ReSum_inl, resum, ReSum_id, id_. cbn.
+  setoid_rewrite interp_ret.
+  rewrite bind_bind.
+  setoid_rewrite bind_ret.
+  repeat rewrite interp_state_bind.
+  unfold Id_IFun.
+  unfold CategoryOps.cat, Cat_Handler, Handler.cat. cbn.
+  unfold inl_, Inl_sum1_Handler, Handler.inl_, Handler.htrigger.
+  unfold insert.
+  setoid_rewrite interp_trigger. rewrite tau_eutt.
+  repeat rewrite interp_state_trigger.  cbn.
+  rewrite tau_eutt.
+  setoid_rewrite interp_state_ret.
+  rewrite bind_ret. cbn.
+  reflexivity.
+Qed.  
+
+Lemma interp_asm_Load {E A} f a mem reg :
+  @eutt E _ _ (@rel_asm A)
+       (interp_asm (val <- trigger (Load a) ;; f val) mem reg)
+       ((interp_asm (f (lookup_default a 0 mem))) mem reg).
+Proof.
+  unfold interp_asm, run_map.
+  rewrite interp_bind.
+  rewrite interp_trigger. rewrite tau_eutt.
+  unfold subevent, resum, ReSum_inr, resum, ReSum_inl, resum, ReSum_id, id_. cbn.
+  repeat rewrite interp_state_bind.
+  unfold Id_IFun.
+  unfold CategoryOps.cat, Cat_Handler, Handler.cat. cbn.
+  unfold CategoryOps.cat, Cat_Handler, Handler.cat. cbn.
+  unfold inl_, Inl_sum1_Handler, Handler.inl_, Handler.htrigger.
+  unfold inr_, Inr_sum1_Handler, Handler.inr_, Handler.htrigger.
+  unfold lookup_def.
+  rewrite interp_bind.
+  setoid_rewrite interp_trigger. rewrite tau_eutt.
+  setoid_rewrite interp_ret.
+  rewrite interp_bind. repeat rewrite interp_trigger. rewrite tau_eutt.
+  setoid_rewrite interp_ret.
+  repeat rewrite interp_state_bind.
+  repeat setoid_rewrite interp_state_ret.
+  repeat rewrite interp_state_trigger. rewrite tau_eutt.
+  cbn. unfold pure_state. rewrite interp_state_vis. cbn.  rewrite tau_eutt.
+  rewrite bind_ret. rewrite interp_state_ret.
+  repeat rewrite bind_ret. cbn. 
+  unfold lookup_default.
+  unfold lookup, Map_alist. reflexivity.
+Qed.  
+
+Lemma interp_asm_Store {E A} f a v mem reg :
+  @eutt E _ _ (@rel_asm A)
+       (interp_asm (trigger (Store a v) ;; f) mem reg)
+       ((interp_asm f) (Maps.add a v mem) reg).
+Proof.
+  unfold interp_asm, run_map.
+  rewrite interp_bind.
+  rewrite interp_trigger. rewrite tau_eutt.
+  unfold subevent, resum, ReSum_inr, resum, ReSum_inl, resum, ReSum_id, id_. cbn.
+  repeat rewrite interp_state_bind.
+  unfold Id_IFun.
+  unfold CategoryOps.cat, Cat_Handler, Handler.cat. cbn.
+  unfold CategoryOps.cat, Cat_Handler, Handler.cat. cbn.
+  unfold inl_, Inl_sum1_Handler, Handler.inl_, Handler.htrigger.
+  unfold inr_, Inr_sum1_Handler, Handler.inr_, Handler.htrigger.
+  unfold insert, embed, Embeddable_forall, embed, Embeddable_itree. 
+  rewrite interp_trigger. rewrite tau_eutt.
+  setoid_rewrite interp_trigger. rewrite tau_eutt.
+  rewrite interp_state_trigger. rewrite tau_eutt. cbn.
+  unfold pure_state. rewrite interp_state_vis. cbn.  rewrite tau_eutt.
+  rewrite bind_ret. rewrite interp_state_ret.
+  repeat rewrite bind_ret. cbn. 
+  reflexivity.
+Qed.  
+  
 
 
 (* peephole optimizations --------------------------------------------------- *)
@@ -89,51 +390,111 @@ Section Correctness.
     a semantically equivalent sequence of instructions. *)
   Definition ph_correct (ph : peephole_optimization) :=
   forall (i:instr),
-    @eq_asm_denotations Exit unit _ (fun _ => denote_instr i) (fun _ => denote_list (ph i)).
+    @eq_asm_denotations_EQ Exit unit _ (fun _ => denote_instr i) (fun _ => denote_list (ph i)).
 
   Lemma ph_blk_append_correct : forall (ph : peephole_optimization) (H : ph_correct ph)
     lbl1 lbl2 b1 b2 i,
-    (@eq_asm_denotations Exit (F lbl1) (F lbl2) (fun _ => denote_block b1) (fun _ => denote_block b2)) ->
-    (@eq_asm_denotations Exit (F lbl1) (F lbl2)
+    (@eq_asm_denotations_EQ Exit (F lbl1) (F lbl2) (fun _ => denote_block b1) (fun _ => denote_block b2)) ->
+    (@eq_asm_denotations_EQ Exit (F lbl1) (F lbl2)
                          (fun _ => denote_instr i ;; denote_block b1)
                          (fun _ => denote_block (blk_append (ph i) b2))).
   Proof.
     intros ph H lbl1 lbl2 b1 b2 i HP.
-    unfold eq_asm_denotations.
-    intros a mem regs. 
+    unfold eq_asm_denotations_EQ.
+    intros a mem1 mem2 regs1 regs2 EQ_mem EQ_reg.
     rewrite denote_blk_append.
     unfold ph_correct in H.
-    unfold eq_asm_denotations in H.
+    unfold eq_asm_denotations_EQ in H.
     specialize H with (i:=i).
     pose proof (H tt) as H2.
     do 2 rewrite interp_asm_bind.
     eapply eutt_clo_bind.
-    apply H2.
-    intros. subst.
-    destruct u2 as [g [l ?]].
-    apply HP.
-    exact a.
+    apply H2; auto.
+    intros. 
+    inversion H0.
+    apply HP; auto.
   Qed.  
 
+  Lemma EQ_registers_lookup : forall regs1 regs2 r ,
+      EQ_registers regs1 regs2 ->
+      lookup r regs1 = lookup r regs2.
+  Proof.
+    intros. unfold EQ_registers, alist_In in H.
+    unfold lookup, Map_alist.
+    remember (alist_find r regs1) as x.
+    destruct x.
+    - symmetry in Heqx. rewrite H in Heqx. rewrite Heqx. reflexivity.
+    - remember (alist_find r regs2) as x.
+      destruct x.
+      symmetry in Heqx0. rewrite <- H in Heqx0. rewrite Heqx0 in Heqx. inversion Heqx.
+      reflexivity.
+ Qed.
+    
+Lemma EQ_registers_lookup_default : forall regs1 regs2 r v,
+      EQ_registers regs1 regs2 ->
+      lookup_default r v regs1 = lookup_default r v regs2.
+Proof.
+  intros regs1 regs2 r v H.
+  unfold lookup_default.
+  erewrite EQ_registers_lookup. reflexivity. assumption.
+Qed.
+  
 
 Lemma peephole_block_correct : 
   forall (ph : peephole_optimization)
     (H : ph_correct ph)
     (lbl1 lbl2 : nat)
     (b : block (F lbl2)),
-    @eq_asm_denotations Exit (F lbl1) (F lbl2)
+    @eq_asm_denotations_EQ Exit (F lbl1) (F lbl2)
                         (fun _ => denote_block b)
                         (fun _ => denote_block (peephole_optimize_block ph b)).
 Proof.
   intros ph H lbl1 lbl2 b.
   induction b.
   - simpl.
-    unfold eq_asm_denotations.
+    unfold eq_asm_denotations_EQ.
     intros.
-    eapply ph_blk_append_correct. assumption. exact IHb. assumption.
-  - unfold eq_asm_denotations.
-    intros. reflexivity.
-Qed.    
+    eapply ph_blk_append_correct; try assumption. exact IHb. assumption.
+  - unfold eq_asm_denotations_EQ.
+    intros. 
+    destruct b; simpl.
+    + unfold interp_asm.
+      rewrite interp_ret.
+      unfold run_map.
+      repeat rewrite interp_state_ret.
+      apply eqit_Ret. constructor; auto.
+    + setoid_rewrite interp_asm_GetReg.
+      rewrite (EQ_registers_lookup_default _ regs2); auto.
+      unfold value in *.
+      remember (lookup_default r 0 regs2) as x.
+      destruct x.
+      repeat rewrite interp_asm_ret.
+      apply eqit_Ret. constructor; auto.
+      repeat rewrite interp_asm_ret.
+      apply eqit_Ret. constructor; auto.
+    + unfold interp_asm, run_map.
+      unfold id_, Id_Handler, Handler.id_.
+      unfold exit.
+      rewrite interp_vis. rewrite tau_eutt.
+      cbn. rewrite interp_state_bind.
+      unfold CategoryOps.cat, Cat_Handler, Handler.cat, inr_, Inr_sum1_Handler, Handler.inr_, Handler.htrigger.
+      setoid_rewrite interp_trigger. rewrite tau_eutt.
+      unfold inr_.
+      rewrite interp_trigger. rewrite tau_eutt.
+      rewrite interp_state_trigger. rewrite tau_eutt.
+      rewrite interp_state_bind.
+      cbn. unfold pure_state. rewrite interp_state_vis. cbn.  rewrite tau_eutt.
+      repeat rewrite bind_vis.
+      rewrite interp_state_bind.
+      rewrite interp_state_trigger. cbn.  rewrite tau_eutt.
+      rewrite bind_vis.
+      rewrite interp_state_vis. rewrite tau_eutt. cbn.
+      rewrite bind_vis.
+      unfold resum, ReSum_id, id_, Id_IFun.
+      apply eqit_Vis.
+      intros. inversion u.
+Qed.
+
 
 Lemma peephole_optimization_correct : forall A B (ph : peephole_optimization) (H : ph_correct ph),
     optimization_correct A B (peephole_optimize_asm ph).
@@ -142,49 +503,77 @@ Proof.
   unfold optimization_correct.
   intros p.
   unfold eq_asm, eq_asm_denotations, denote_asm.
-  intros a mem regs.
+  intros a mem1 mem2 regs1 regs2 H1 H2.
   unfold interp_asm, run_map.
   repeat setoid_rewrite interp_bind.
   repeat rewrite interp_state_bind.
-  eapply eutt_clo_bind.
-  { reflexivity. }
-  intros. simpl in *.
-  rewrite H0.
-  destruct u2 as [mem' [regs' z]].
-  simpl.
+  apply (@eutt_clo_bind _ _ _ _ _ _ rel_asm).
+
+  
+  { apply (@eutt_clo_bind _ _ _ _ _ _ rel_asm).
+    -  unfold inr_, CoprodInr_Kleisli, lift_ktree_.
+       unfold ret, Monad_itree.
+       repeat rewrite interp_ret.
+       repeat rewrite interp_state_ret.
+       apply eqit_Ret. constructor; auto.
+    -  intros. inversion H0.
+       subst. cbn.
+       repeat rewrite interp_ret.
+       repeat rewrite interp_state_ret.
+       apply eqit_Ret. constructor; auto. }
+    
+  intros. 
+  inversion H0.
+  subst. simpl in *.
   unfold denote_b.
   unfold iter, Iter_sktree.
   repeat rewrite interp_iter.
   unfold KTree.iter, Iter_ktree.
   cbn. 
   pose proof @interp_state_aloop'.
-  red in H1.
-  repeat rewrite H1.
+  red in H3.
+  repeat rewrite H3.
   unfold aloop, ALoop_stateT0, aloop, ALoop_itree.
-  repeat rewrite H1.
+  repeat rewrite H3.
   unfold aloop, ALoop_stateT0, aloop, ALoop_itree.
-  eapply (@eutt_aloop'  _ _ _ _ _ eq); auto.
-  intros j1 j2 Heq.
-  rewrite Heq.
-  destruct j2 as [mem'' [regs'' [ll | rr]]]; cbn.
+  eapply (@eutt_aloop'  _ _ _ _ _ rel_asm); auto.
+  intros j1 j2 Hrel.
+  inversion Hrel.
+  subst; cbn.
+  destruct b0.
   - constructor.
     repeat rewrite interp_bind.
     repeat rewrite interp_state_bind.
-    eapply eutt_clo_bind.
-    + eapply eutt_clo_bind.
+    eapply (@eutt_clo_bind _ _ _ _ _ _ rel_asm).
+    + eapply (@eutt_clo_bind _ _ _ _ _ _ rel_asm).
       * unfold peephole_optimize_bks.
         pose proof @peephole_block_correct.
-        unfold eq_asm_denotations, interp_asm, run_map in H2.    
-        eapply H2.
-        apply H.
-        apply ll.
+        unfold eq_asm_denotations_EQ, interp_asm, run_map in H4.    
+        eapply H4; auto.
+        apply f.
       * intros.
-        rewrite H2.
-        reflexivity.
+        inversion H4.
+        subst. cbn.
+        repeat rewrite bind_ret.
+        unfold CategoryOps.cat, Cat_sktree, CategoryOps.cat, Cat_Kleisli. cbn.
+        unfold case_, Case_sum1, CoprodCase_Kleisli, case_sum.
+        destruct (split_fin_sum b0).
+        -- repeat rewrite bind_ret.
+           rewrite interp_ret.
+           repeat rewrite interp_state_ret.
+           apply eqit_Ret. constructor; auto.
+        -- repeat rewrite bind_ret.
+           rewrite interp_ret.
+           repeat rewrite interp_state_ret.
+           apply eqit_Ret. constructor; auto.
     + intros.
-      rewrite H2.
-      reflexivity.
-  - constructor. reflexivity.
+      inversion H4.
+      subst; cbn.
+      rewrite interp_ret.
+      repeat rewrite interp_state_ret.
+      apply eqit_Ret. constructor; auto.
+  - constructor. constructor; auto.
+  - constructor; auto.
 Qed.    
 
 
@@ -198,77 +587,106 @@ Definition simple (i:instr) : list instr :=
   end.
 
 
-Lemma interp_asm_ret_tt : forall (t : itree (Reg +' Memory +' Exit) unit) mem regs,
-    interp_asm t mem regs ≈ interp_asm (t ;; Ret tt) mem regs.
-Proof.
-  intros t mem regs.
-  rewrite interp_asm_bind.
-  rewrite <- bind_ret2 at 1.
-  eapply eutt_clo_bind. reflexivity.
-  intros. subst. unfold interp_asm.
-  destruct u2 as [g [l x]].
-  unfold run_map.
-  rewrite interp_ret.
-  do 2 rewrite interp_state_ret.
-  destruct x.
-  reflexivity.
-Qed.
+(* TODO: Move to utilities *)
+Section alist_facts.
 
+  Context {K V: Type}.
+  Context {RR : @RelDec K (@eq K)}.
+  Context {RRC : @RelDec_Correct K (@eq K) RR}.
+
+  Lemma alist_In_add_eq : forall m (k:K) (v n:V), alist_In k (alist_add k n m) v -> n = v.
+  Proof.
+    destruct m as [| [k1 v1]]; intros.
+    - unfold alist_add in H.
+      unfold alist_In in H. simpl in H.
+      destruct (k ?[ eq ] k); inversion H; auto.
+    - unfold alist_add in H.
+      unfold alist_In in H.
+      simpl in H.
+      destruct (k ?[ eq ] k). inversion H; auto.
+      pose proof (@not_In_remove K V _ _ ((k1,v1)::m)).
+      unfold alist_In in H0. simpl in H0.
+      apply H0 in H.
+      contradiction.
+  Qed.
+End alist_facts.
+
+  
+(* SAZ: Belongs in the utilities? (but depends on EQ_registers) *)
+Lemma EQ_registers_add:
+  forall (r : reg) (regs1 regs2 : registers),
+    EQ_registers regs1 regs2 ->
+    EQ_registers (alist_add r (lookup_default r 0 regs1) regs1) regs2.
+Proof.
+  intros r regs1 regs2 H.
+  unfold EQ_registers in *.
+  intros.
+  unfold lookup_default, lookup, Map_alist.
+  remember (@alist_find reg _ RelDec_reg nat r regs1) as x.
+  unfold alist_In.
+  unfold alist_add.
+  destruct x; simpl in *.
+  unfold rel_dec, RelDec_reg; simpl.
+  - destruct (Nat.eq_dec k r).
+    + subst.
+      split; intros.
+      inversion H0. subst.
+      unfold alist_In in H.
+      apply H. symmetry. assumption.
+      unfold alist_In in H.
+      unfold value in *.
+      apply H in H0.
+      rewrite H0 in Heqx.
+      assumption.
+
+    + split; intros.
+      unfold alist_In in H0.
+Admitted.
 
 Lemma simple_correct : ph_correct simple.
 Proof.
   unfold ph_correct.
   intros i.
-  unfold eq_asm_denotations. intros. 
-  destruct i; simpl; try apply interp_asm_ret_tt.
-  - destruct src.
-    + simpl. rewrite bind_ret.
-      apply interp_asm_ret_tt. 
-    + simpl.
-      destruct (Nat.eq_dec dest r).
-      * subst. 
-        rewrite Nat.eqb_refl.
-        simpl.
-        unfold interp_asm, run_map.
-        rewrite interp_ret.
-        do 2 rewrite interp_state_ret.
-        rewrite interp_bind.
-        rewrite interp_trigger.
-        rewrite bind_tau.
-        rewrite tau_eutt.
-        do 2 rewrite interp_state_bind.
-        cbn.
-        unfold CategoryOps.cat, Cat_Handler, Handler.cat. simpl.
-        unfold lookup_def.
-        repeat rewrite interp_bind.
-        setoid_rewrite interp_ret.
-        repeat rewrite interp_state_bind.
-        repeat rewrite bind_bind.        
-        repeat setoid_rewrite interp_state_ret.
+  unfold eq_asm_denotations_EQ.
+  intros. 
+  destruct i; simpl; try apply interp_asm_ret_tt; auto; try reflexivity.
 
-        unfold Map.lookup.
-        unfold embed, Embeddable_itree, Embeddable_forall, inl_, embed.
-        rewrite interp_trigger. rewrite tau_eutt.
-        unfold Inl_sum1_Handler, Handler.inl_, Handler.htrigger.
-        rewrite interp_state_trigger. rewrite tau_eutt.
-        cbn.
-        rewrite interp_state_ret.
-        repeat rewrite bind_ret.
-        simpl.
-        rewrite interp_trigger.
-        rewrite tau_eutt.
-        cbn. 
-        unfold CategoryOps.cat, resum, ReSum_id, id_, eval_reg, inl_. cbn.
-        setoid_rewrite interp_trigger. rewrite tau_eutt.
-        rewrite interp_state_trigger.
-        rewrite tau_eutt.
-        cbn.
-        rewrite interp_state_ret.
+  destruct src.
+  + simpl. rewrite bind_ret.
+    apply interp_asm_ret_tt; auto; try reflexivity.
 
-        (* SAZ: need to propagate an equivalence relation on the register state. *)
+  + simpl.
+    destruct (Nat.eq_dec dest r).
+    * subst. 
+      rewrite Nat.eqb_refl.
+      simpl.
+      rewrite interp_asm_ret.      
+      rewrite interp_asm_GetReg.
 
-        
-Admitted.    
-
+      unfold trigger.
+      unfold interp_asm, run_map.
+      rewrite interp_vis. rewrite tau_eutt.
+      cbn.
+      repeat rewrite interp_state_bind.
+      unfold CategoryOps.cat, Cat_Handler, Handler.cat. simpl.
+      unfold inl_, Inl_sum1_Handler, Handler.inl_, Handler.htrigger.
+      unfold insert.
+      unfold embed, Embeddable_itree, Embeddable_forall, inl_, embed.
+      rewrite interp_trigger. rewrite tau_eutt.
+      rewrite interp_state_trigger. rewrite tau_eutt.
+      cbn.
+      rewrite interp_state_ret.
+      rewrite bind_ret.
+      rewrite interp_ret.
+      repeat rewrite interp_state_ret.
+      cbn.
+      apply eqit_Ret.
+      constructor; auto.
+      apply EQ_registers_add; auto.
+    * apply Nat.eqb_neq in n.
+      rewrite n.
+      simpl.
+      apply interp_asm_ret_tt; auto. reflexivity.
+Qed.      
 
 End Correctness.
